theories/zoo/program_logic/counter.v
@@ -5,8 +5,6 @@ From zoo Require Import
   prelude.
 From zoo.iris.bi Require Import
   big_op.
-From zoo.iris.base_logic Require Import
-  lib.mono_list.
 From zoo.language Require Import
   notations.
 From zoo.program_logic Require Export
@@ -23,29 +21,6 @@ Definition zoo_counter_incr : val :=
 Section zoo_G.
   Context `{zoo_G : !ZooG Σ}.
 
-  Definition zoo_counter_at :=
-    mono_list_at (mono_list_G := zoo_G_counter_G) zoo_counter_name.
-
-  #[global] Instance zoo_counter_at_timeless id v :
-    Timeless (zoo_counter_at id v).
-  Proof.
-    apply _.
-  Qed.
-
-  #[global] Instance zoo_counter_at_persistent id v :
-    Persistent (zoo_counter_at id v).
-  Proof.
-    apply _.
-  Qed.
-
-  Lemma zoo_counter_at_agree id v1 v2 :
-    zoo_counter_at id v1 -∗
-    zoo_counter_at id v2 -∗
-    ⌜v1 = v2⌝.
-  Proof.
-    apply mono_list_at_agree.
-  Qed.
-
   Lemma zoo_counter_incr_spec ids v :
     {{{
       [∗ list] id ∈ ids,
@@ -61,7 +36,7 @@ Section zoo_G.
   Proof.
     iIntros "%Φ Hids HΦ".
 
-    iApply wp_state_interp. iIntros "%nt %σ %κs Hinterp !>".
+    iApply wp_state_interp. iIntros "%ns %nt %σ %κs Hinterp !>".
     iDestruct (state_interp_counter_inv with "Hinterp") as "#Hinv".
     iFrame.
 
@@ -74,15 +49,13 @@ Section zoo_G.
     iAssert ⌜Forall (.≠ length vs) ids⌝%I as "%Hids".
     { rewrite Forall_lookup. iIntros "%i %id %Hlookup".
       iDestruct (big_sepL_lookup with "Hids") as "(%w & Hat)"; first done.
-      iDestruct (mono_list_at_valid with "Hauth Hat") as %Hid%lookup_lt_Some.
+      iDestruct (zoo_counter_at_valid with "Hauth Hat") as %Hid%lookup_lt_Some.
       iSteps.
     }
 
-    iMod (mono_list_update_snoc v with "Hauth") as "Hauth".
-    iDestruct (mono_list_at_get with "Hauth") as "#Hat".
+    iMod (zoo_counter_update v with "Hauth") as "Hauth".
+    iDestruct (zoo_counter_at_get with "Hauth") as "#Hat".
     { apply list_lookup_middle. done. }
     iSteps. iPureIntro. simpl_length/=. lia.
   Qed.
 End zoo_G.
-
-#[global] Opaque zoo_counter_at.
